case_study/RiscvPmp/CFGVer/Examples.v
@@ -331,15 +331,15 @@ Module Examples.
 
   Search Assertion.
 
-  Definition asn_regs_ptsto_with_registers {Σ} γ1 γ2 : Assertion Σ :=
+  Definition asn_regs_ptsto_with_registers γ1 γ2 : Assertion ctx.nil :=
     asn_and_regs
       (fun r => asn.chunk (chunk_ptsreg r (term_relval _ (NonSyncVal (read_register γ1 r) (read_register γ2 r))))).
 
-  Lemma gprs_with_registers_equiv `{sailGS2 Σ} γ1 γ2 : ∀ {Σ} (ι : Valuation Σ),
+  Lemma gprs_with_registers_equiv `{sailGS2 Σ} γ1 γ2 :
       interp_gprs_with_registers γ1 γ2 ⊣⊢
-        asn.interpret (asn_regs_ptsto_with_registers γ1 γ2) ι.
+        asn.interpret (asn_regs_ptsto_with_registers γ1 γ2) env.nil.
   Proof.
-    iIntros. unfold interp_gprs_with_registers.
+    unfold interp_gprs_with_registers.
     rewrite big_sepS_list_to_set; [|apply bv.finite.nodup_enum].
     cbn. iSplit.
     - iIntros "(_ & H)"; repeat iDestruct "H" as "($ & H)".
@@ -1120,7 +1120,6 @@ End AdequacyTools.
       destruct an as [v | v1 v2].
       + cbn in Hexit. left. cbn. rewrite Hexit. exact I.
       + contradiction.
-    Unshelve. all: try exact R. all: try exact ι.
   Qed.
 
   Lemma cfg_instrs_safe `{sailGS2 Σ} instrs' exitCond γ1 γ2 {R} {ι : Valuation R}
@@ -1258,7 +1257,6 @@ End AdequacyTools.
       repeat (iDestruct "Hregs" as "($ & Hregs)").
       auto.
     - cbn. by unfold lenAddr.
-    Unshelve. exact ctx.nil. exact env.nil.
   Qed.
 
   Lemma jumpIfZero_endToEnd {γ1 γ2 γ1' γ2' : RegStore} {μ1 μ2 μ1' μ2' : Memory} n ws
@@ -1296,7 +1294,6 @@ End AdequacyTools.
       iDestruct "Hregs" as "($ & Hregs)".
       done.
     - cbn. by unfold lenAddr.
-    Unshelve. exact ctx.nil. exact env.nil.
   Qed.
 
   Lemma jmp_fwd_safe_cfg `{sailGS2 Σ} γ1 γ2 :
